Cslib/Computability/Machines/MultiTapeTuring/PushRoutine.lean
@@ -6,9 +6,6 @@ Authors: Christian Reitwiessner
 
 module
 
-import Cslib.Foundations.Data.BiTape
-import Cslib.Foundations.Data.RelatesInSteps
-
 public import Cslib.Computability.Machines.MultiTapeTuring.Basic
 public import Cslib.Computability.Machines.MultiTapeTuring.ListEncoding
 public import Cslib.Computability.Machines.MultiTapeTuring.WithTapes
@@ -29,23 +26,16 @@ public lemma push₁_eval_list {w : List α} {tapes : Fin 1 → List (List α)} 
   (push₁ w).eval_list tapes = .some (Function.update tapes 0 (w :: (tapes 0))) := by
   sorry
 
-public def push {k : ℕ} (i : Fin k.succ) (w : List α) : MultiTapeTM k.succ (WithSep α) :=
-  (push₁ w).with_tapes [i].get (by intro x y; grind) (h_le := by omega)
+public def push {k : ℕ} (i : Fin k) (w : List α) : MultiTapeTM k (WithSep α) :=
+  (push₁ w).with_tapes [i].get (by intro x y; grind)
 
 @[simp, grind =]
 public theorem push_eval_list {k : ℕ}
   {i : Fin k.succ} {w : List α} {tapes : Fin k.succ → List (List α)} :
   (push i w).eval_list tapes =
     .some (Function.update tapes i (w :: (tapes i))) := by
-  simp [push]
-  grind
-
--- public lemma push₁_evalWithStats_list {w : List α} {ls : List (List α)} :
---   (push₁ w).evalWithStats_list #v[ls].get =
---     .some (
---       [w :: ls].get,
---       [⟨-w.length - 1, 0, -w.length - 1, by omega⟩].get) := by
---   sorry
+  have h_inj : [i].get.Injective := by intro x y; grind
+  simp_all [push]
 
 end Routines
 
